Makefile
@@ -1,5 +1,5 @@
 pdf:
-	isabelle build -d . -d Word_Lib -v cap9-spec
+	isabelle build -d . -v cap9-spec
 
 html:
 	isabelle build -d . -o browser_info -v cap9-spec
